WIP: CAproof, leaving internal steps

demo/DemoBproofnew.v
@@ -20,14 +20,240 @@ Search wt_c.
 
 Section injp_CA.
 
-Lemma injp_CA: forward_simulation
+Section MS.
+Variable w: ccworld (cc_c injp @ cc_c_asm).
+
+Definition se := fst (fst w).
+Definition injw := snd (fst w).
+Definition caw0 := snd (w).
+Definition sg := caw_sg caw0.
+Definition rs0 := caw_rs caw0.
+Definition m2 := caw_m caw0.
+
+Definition sp0 := rs0 RSP.
+Definition ra0 := rs0 RA.
+Definition vf0 := rs0 PC.
+Definition bx0 := rs0 RBX. (*only used callee_save register in this sample*)
+(*cc_c_asm_mq*)
+
+Inductive new_blockv (s:sup) : val -> Prop :=
+  new_blockv_intro : forall b ofs, ~ sup_In b s -> new_blockv s (Vptr b ofs).
+
+Inductive match_state_c_asm : state -> (sup * Asm.state) -> Prop :=
+  |match_ca_callg i m m2':
+     injp_match_mem injw m m2' ->
+     args_removed sg sp0 m2 m2 ->
+     rs0 RDI = Vint i ->
+     match_state_c_asm (Callstateg i m) ((Mem.support m2),State rs0 m2 true)
+  |match_ca_callf w' i m m2' tm (rs: regset) vfc sb:
+     let sp := rs RSP in let ra := rs RA in let vf := rs PC in
+     injp_acc injw w' ->
+     injp_match_mem w' m m2' ->
+     rs RBX = Vint i ->
+     rs RDI = Vint (Int.sub i Int.one) ->
+     args_removed int_int_sg sp tm m2' ->
+     Val.has_type sp Tptr -> Val.has_type ra Tptr ->
+     sp = Vptr sb Ptrofs.zero ->
+     sup_In sb (Mem.support tm) -> ~ sup_In sb (Mem.support m2) ->
+     (forall i, loc_out_of_reach (injp_mi w') m sb i) ->
+     vf <> Vundef -> ra <> Vundef -> vfc <> Vundef ->
+     Val.inject (injp_mi w') vfc vf ->
+     Mem.loadv Mptr tm (Val.offset_ptr sp (Ptrofs.repr 16)) = Some ra0 ->
+     Mem.loadv Mptr tm (Val.offset_ptr sp Ptrofs.zero) = Some sp0 ->
+     Mem.loadv Many64 tm (Val.offset_ptr sp (Ptrofs.repr 8)) = Some bx0 ->
+     (forall r, is_callee_save r = true /\ r <> BX -> rs (preg_of r) = rs0 (preg_of r)) ->
+     Mem.sup_include (Mem.support m2) (Mem.support tm) -> (*unchanged_on of Outgoing*)
+     match_state_c_asm (Callstatef vfc i m) ((Mem.support m2),State rs tm true)
+  |match_ca_returnf w' m2' i rig m tm (rs: regset):
+     let sp := rs RSP in
+     injp_acc injw w' ->
+     injp_match_mem w' m m2' ->
+     rs RBX = Vint i -> rs RAX = Vint rig ->
+     Mem.unchanged_on (fun b ofs => True) m2' tm ->
+     Mem.support m2' = Mem.support tm ->
+     Mem.loadv Mptr tm (Val.offset_ptr sp (Ptrofs.repr 16)) = Some ra0 ->
+     Mem.loadv Mptr tm (Val.offset_ptr sp Ptrofs.zero) = Some sp0 ->
+     Mem.loadv Many64 tm (Val.offset_ptr sp (Ptrofs.repr 8)) = Some bx0 ->
+     (forall r, is_callee_save r = true /\ r <> BX -> rs (preg_of r) = rs0 (preg_of r)) ->
+     Mem.sup_include (Mem.support m2) (Mem.support tm) -> (*unchanged_on of Outgoing*)
+     match_state_c_asm (Returnstatef i rig m) ((Mem.support m2), State rs tm true)
+  |match_ca_returng w' m2' m tm (rs: regset) ri:
+     injp_acc injw w' ->
+     injp_match_mem w' m m2' ->
+     rs RAX = Vint ri ->
+     Mem.unchanged_on (fun b ofs => True) m2' tm ->
+     Mem.support m2' = Mem.support tm ->
+     rs RSP = rs0 RSP -> rs PC = rs0 RA ->
+     (forall r, is_callee_save r = true -> rs (preg_of r) = rs0 (preg_of r)) ->
+     Mem.sup_include (Mem.support m2) (Mem.support tm) -> (*unchanged_on of Outgoing*)
+     (*cc_c_asm_mr*)
+     match_state_c_asm (Returnstateg ri m) ((Mem.support m2), State rs tm false).
+End MS.
+
+Axiom not_win: Archi.win64 = false.
+Lemma size_int_int_sg_0:
+  size_arguments int_int_sg = 0.
+Proof.
+  unfold size_arguments, int_int_sg, loc_arguments. replace Archi.ptr64 with true by reflexivity.
+  rewrite not_win. reflexivity.
+Qed.
+
+Lemma loc_arguments_int :
+  loc_arguments int_int_sg = One (R DI)::nil.
+Proof.
+  unfold loc_arguments.
+  replace Archi.ptr64 with true by reflexivity.
+  rewrite not_win. simpl. reflexivity.
+Qed.
+
+Lemma loc_result_int :
+  loc_result int_int_sg = One AX.
+Proof.
+  unfold loc_result.
+  replace Archi.ptr64 with true by reflexivity.
+  reflexivity.
+Qed.
+
+Lemma match_program_id :
+  match_program (fun _ f0 tf => tf = id f0) eq prog prog.
+Proof.
+  red. red. constructor; eauto.
+    constructor. constructor. eauto. simpl. econstructor; eauto.
+    apply linkorder_refl.
+    constructor. constructor; eauto. constructor; eauto.
+    constructor; eauto.
+    constructor; eauto. constructor; eauto. simpl. econstructor; eauto.
+    apply linkorder_refl.
+    constructor.
+Qed.
+
+Lemma loadv_unchanged_on : forall P m m' chunk b ptrofs v,
+    Mem.unchanged_on P m m' ->
+    (forall i, let ofs := Ptrofs.unsigned ptrofs in
+    ofs <= i < ofs + size_chunk chunk -> P b i) ->
+    Mem.loadv chunk m (Vptr b ptrofs) = Some v ->
+    Mem.loadv chunk m' (Vptr b ptrofs) = Some v.
+Proof.
+  intros. unfold Mem.loadv in *. cbn in *.
+  eapply Mem.load_unchanged_on; eauto.
+Qed.
+
+Lemma injp_CA_simulation: forward_simulation
                  (cc_c injp @ cc_c_asm)
                  (cc_c injp @ cc_c_asm)
                  Bspec (Asm.semantics prog).
 Proof.
- Admitted.
+  constructor. econstructor; eauto. instantiate (1 := fun _ _ _ => _). cbn beta.
+  intros se1 se2 w Hse Hse1. cbn in *. subst.
+  pose (ms := fun s1 s2 => match_state_c_asm w s1 s2 /\
+                         caw_sg (snd w) = int_int_sg).
+  eapply forward_simulation_plus with (match_states := ms);
+  destruct w as [[se [f ? ? Hm]] [sg rs0 m2'0]]; destruct Hse; subst; cbn in *; eauto.
+  - (*valid_query*)
+    intros. destruct H0 as [qm [Hq1 Hq2]]. inv Hq1. inv Hq2.
+    simpl. cbn in *. subst vf.
+    generalize  match_program_id. intro TRAN.
+    eapply Genv.is_internal_transf in TRAN; eauto. inv H; eauto.
+  - (* initial *)
+    intros q1 q3 s1 [q2 [Hq1 Hq2]] Hi1. inv Hi1.
+    inv Hq1. inv Hq2. cbn in *. inv H7.
+    exists (Mem.support m2'0, State rs0 m2'0 true). repeat apply conj.
+    + econstructor; eauto.
+      generalize  match_program_id. intro TRAN.
+      eapply Genv.find_funct_transf in TRAN; eauto. inv H; eauto.
+      inv H17. subst sp. congruence.
+    + eauto.
+    + econstructor; cbn; eauto.
+      constructor. red. rewrite size_int_int_sg_0. reflexivity.
+      rewrite loc_arguments_int in H6. simpl in H6. inv H6. inv H3. reflexivity.
+    + eauto.
+  - (* final_state *)
+    intros s1 s3 r1 Hms Hf1. inv Hf1. inv Hms. inv H0. cbn in *.
+    exists (rs,tm). split. constructor.
+    exists (cr (Vint s) m2'). split.
+    exists w'. split. eauto. constructor; eauto.
+    constructor; eauto. eapply Mem.unchanged_on_implies; eauto.
+    intros. simpl. auto.
+    constructor. eauto with mem.
+    intros. inv H0. rewrite size_int_int_sg_0 in H11. extlia.
+    intros. inv H0. rewrite size_int_int_sg_0 in H11. extlia.
+    intros. inv H0. rewrite size_int_int_sg_0 in H2. extlia.
+  - (* at_external*)
+    intros s1 s2 q1 MS EXT1. inv EXT1. inv MS.
+    inv H0. cbn in *. inv H4. inv H5. cbn in *.
+    inv H. eapply Genv.match_stbls_incr in H4; eauto.
+    2:{
+      intros. exploit H29; eauto. intros [A B].
+      unfold Mem.valid_block in *. split; eauto with mem.
+    }
+    exists ((se2,(injpw f' m m2' Hm4)),(caw int_int_sg rs tm)).
+    exists (rs,tm). repeat apply conj.
+    + econstructor; eauto.
+      generalize  match_program_id. intro TRAN.
+      eapply Genv.find_funct_transf in TRAN; eauto.
+    + exists (cq vf1 int_int_sg (Vint (Int.sub aif Int.one)::nil) m2').
+      split.
+      -- constructor; eauto. simpl. constructor.
+      -- econstructor; eauto.
+         rewrite loc_arguments_int. simpl. congruence.
+         subst sp. rewrite H11. constructor; eauto.
+    + constructor. apply H4.
+      inversion H25. eauto with mem.
+      inversion H26. eauto with mem.
+    + reflexivity.
+    + (*after_external*)
+      intros r1 r3 s1' [r2 [Hr1 Hr2]] Haf1.
+      destruct Hr1 as [w [Hw Hr1]]. inv Haf1. inv Hr1. inv Hr2.
+      cbn in *.
+      exists ((Mem.support m2'0), (State rs' tm' true)). repeat apply conj.
+      -- constructor. inversion H36; eauto.
+         unfold inner_sp. rewrite H40. subst sp. rewrite H11.
+         rewrite pred_dec_false; eauto.
+      -- reflexivity.
+      -- econstructor; cbn.
+         ++ etransitivity; eauto. constructor; eauto.
+         ++ eauto.
+         ++ generalize (H34 BX). intro. exploit H; eauto.
+            simpl. intro A. rewrite A. eauto.
+         ++ rewrite loc_result_int in H1. simpl in H1.
+            inv H1. reflexivity.
+         ++ eapply Mem.unchanged_on_implies; eauto.
+            intros. red. intro. inv H2. rewrite size_int_int_sg_0 in H32. extlia.
+         ++ eauto.
+         ++ destruct w. inv H5. inv Hw.
+            rewrite H40. subst sp. rewrite H11 in *. cbn in *.
+            eapply Mem.load_unchanged_on. apply H35.
+            intros. simpl. red. intro A. inv A. rewrite size_int_int_sg_0 in H2. extlia.
+            eapply Mem.load_unchanged_on. apply H43.
+            intros. eauto.
+            inv H8. eauto.
+            rewrite size_int_int_sg_0 in H27. extlia.
+         ++ destruct w. inv H5. inv Hw.
+            rewrite H40. subst sp. rewrite H11 in *. cbn in *.
+            eapply Mem.load_unchanged_on. apply H35.
+            intros. simpl. red. intro A. inv A. rewrite size_int_int_sg_0 in H2. extlia.
+            eapply Mem.load_unchanged_on. apply H43.
+            intros. eauto.
+            inv H8. eauto.
+            rewrite size_int_int_sg_0 in H27. extlia.
+         ++ destruct w. inv H5. inv Hw.
+            rewrite H40. subst sp. rewrite H11 in *. cbn in *.
+            eapply Mem.load_unchanged_on. apply H35.
+            intros. simpl. red. intro A. inv A. rewrite size_int_int_sg_0 in H2. extlia.
+            eapply Mem.load_unchanged_on. apply H43.
+            intros. eauto.
+            inv H8. eauto.
+            rewrite size_int_int_sg_0 in H27. extlia.
+         ++ intros. rewrite H34. rewrite H23. eauto. eauto. apply H.
+         ++ inversion H36. eauto with mem.
+      -- reflexivity.
+  - (*internal_steps*)
+    intros. inv H0; inv H1.
+    ++ (*step_zero*)
+      
+      
 
-(*
+End injp_CA.
 Theorem Bproof :
   forward_simulation cc_compcert cc_compcert Bspec (Asm.semantics DemoB.prog).
 Proof.
